HelloTypeSystem/Meta.lean
@@ -8,3 +8,4 @@ import «HelloTypeSystem».Meta.EvalML1
 import «HelloTypeSystem».Meta.TypingML1
 
 import «HelloTypeSystem».Meta.EvalML2
+import «HelloTypeSystem».Meta.TypingML2
